Fixed bugs, added distFilterApp and nullFilter

IntStable.fst
@@ -4,6 +4,7 @@
 **)
 module IntStable
 open FStar.List.Tot
+open FStar.ListProperties
 (*
   This module is heavily inspired by Leino and Lucio's 2012 paper,
   'An Assertional Proof of the Stability and Correctness of Natural Mergesort'.
@@ -28,62 +29,23 @@ let rec filterEq n xs =
 type stable (xs: list int) (ys:list int) = forall x. filterEq x xs = filterEq x ys
 
 (**
-  Several functions and lemmas are needed from FStar.List and FStar.ListProperties
-  These do not load correctly in my binary....
-**)
-
-val append_nil_l: l:list int ->
-  Lemma (requires True)
-        (ensures ([]@l = l))[SMTPat ([]@l)]
-let append_nil_l l = ()
-
-val append_l_nil: l:list int ->
-  Lemma (requires True)
-        (ensures (l@[] = l)) [SMTPat (append l [])]
-let rec append_l_nil = function
-  | [] -> ()
-  | hd::tl -> append_l_nil tl
-
-val append_assoc: l1:list int -> l2:list int -> l3:list int ->
-  Lemma (requires True)
-        (ensures ((l1@(l2@l3)) = ((l1@l2)@l3))) [SMTPat (append l1 (append l2 l3))]
-let rec append_assoc l1 l2 l3 = match l1 with
-    | [] -> ()
-    | hd::tl -> append_assoc tl l2 l3
-
-(* Renamed to avoid conflict *)
-val rev_acc2: list int -> list int -> Tot (list int)
-let rec rev_acc2 l acc = match l with
-    | [] -> acc
-    | hd::tl -> rev_acc2 tl (hd::acc)
-
-val reverseCons: (xs: list int) -> (r: list int) -> (x:int) ->
-  Lemma(requires (xs = rev_acc2 r []))
-    (ensures (append xs (Cons x []) = rev_acc2 (Cons x r) []))
-let reverseCons xs r x =
-  assert(forall a b c. append (rev_acc2 a b) c = rev_acc2 a (append b c))
-
-val flatten: list (list int) -> Tot (list int)
-let rec flatten l = match l with
-    | [] -> []
-    | hd::tl -> append hd (flatten tl)
-
-(**
-  As defined in 'An Assertional Proof...'
-**)
-val flatten_cons_append:
-  (xs: list int)
-  -> (ys: list int)
-  -> (zzs: list (list int))
-  -> Lemma(ensures
-    (flatten (Cons (append xs ys) zzs) = append xs (append ys (flatten zzs))))
-let flatten_cons_append xs ys zzs = ()
-
-
-(**
   Ensures that filtering is distinct with regards to append
 **)
 val distFilterApp: (x: int) -> (xs: list int) -> (ys: list int) ->
   Lemma
   (ensures (filterEq x (append xs ys) = append (filterEq x xs) (filterEq x ys)))
-let distFilterApp x xs ys = ()
+let rec distFilterApp x xs ys =
+  match xs with
+  | [] | [_] -> (match ys with
+    | [] | [_] -> ()
+    | a::b::cs -> distFilterApp x xs (Cons b cs))
+  | a::b::cs -> distFilterApp x (Cons b cs) ys
+
+val nullFilter: (x:int) -> (ys: list int) ->
+  Lemma
+  (requires not (mem x ys))
+  (ensures filterEq x ys = [])
+let rec nullFilter x ys =
+  match ys with
+  | [] | [_] -> ()
+  | a::b::cs -> nullFilter x (Cons b cs)
